@prefix sdl: <https://raw.githubusercontent.com/GX4FM-Base-X/SemanticDataLink/main/oca/overlays/sdlOntology.ttl#> .
@prefix dct: <http://purl.org/dc/terms/> .
@prefix owl: <http://www.w3.org/2002/07/owl#> .
@prefix rdf: <http://www.w3.org/1999/02/22-rdf-syntax-ns#> .
@prefix rdfs: <http://www.w3.org/2000/01/rdf-schema#> .
@prefix xsd: <http://www.w3.org/2001/XMLSchema#> .

sdl: a owl:Ontology ;
    rdfs:label "Semantic Data Link" .

sdl:cardinality
    a owl:DatatypeProperty ;
    rdfs:label "cardinality" ;
    dct:description "Specifies the number of elements in a dataset, often in the context of relationships between data points." ;
    rdfs:domain owl:Class ;
    rdfs:range xsd:string .

sdl:conformance
    a owl:DatatypeProperty ;
    rdfs:label "conformance" ;
    dct:description "Specifies the degree to which the dataset adheres to a standard or specification." ;
    rdfs:domain owl:Class ;
    rdfs:range xsd:string .

sdl:dimensionality
    a owl:DatatypeProperty ;
    rdfs:label "dimensionality" ;
    dct:description "Indicates the number of attributes or fields in the dataset (e.g., columns in a table)." ;
    rdfs:domain owl:Class ;
    rdfs:range xsd:string .

sdl:domain
    a owl:DatatypeProperty ;
    rdfs:label "domain" ;
    dct:description "The field of study or industry to which the dataset is relevant." ;
    rdfs:domain owl:Class ;
    rdfs:range xsd:string .

sdl:encoding
    a owl:DatatypeProperty ;
    rdfs:label "encoding" ;
    dct:description "Details the file encoding format (e.g., UTF-8) used in the dataset." ;
    rdfs:domain owl:Class ;
    rdfs:range xsd:string .

sdl:information
    a owl:DatatypeProperty ;
    rdfs:label "information" ;
    dct:description "A summary of the content and context of the dataset." ;
    rdfs:domain owl:Class ;
    rdfs:range xsd:string .

sdl:keyword
    a owl:DatatypeProperty ;
    rdfs:label "keyword" ;
    dct:description "One of potentially several terms that summarize the main topics or themes of the dataset." ;
    rdfs:domain owl:Class ;
    rdfs:range xsd:string .

sdl:label
    a owl:DatatypeProperty ;
    rdfs:label "label" ;
    dct:description "A human-readable identifier for the dataset or its elements." ;
    rdfs:domain owl:Class ;
    rdfs:range xsd:string .

sdl:size
    a owl:DatatypeProperty ;
    rdfs:label "size" ;
    dct:description "Specifies the total data volume of the dataset, typically in terms of storage space (e.g., MB, GB)." ;
    rdfs:domain owl:Class ;
    rdfs:range xsd:string .

sdl:standard
    a owl:DatatypeProperty ;
    rdfs:label "standard" ;
    dct:description "The technical or domain-specific standard the dataset conforms to." ;
    rdfs:domain owl:Class ;
    rdfs:range xsd:string .

sdl:unit
    a owl:DatatypeProperty ;
    rdfs:label "unit" ;
    dct:description "The measurement unit used within the dataset for quantitative values." ;
    rdfs:domain owl:Class ;
    rdfs:range xsd:string .

sdl:usageFrequency
    a owl:DatatypeProperty ;
    rdfs:label "usage frequency" ;
    dct:description "Indicates how often the dataset is typically accessed or used." ;
    rdfs:domain owl:Class ;
    rdfs:range xsd:string .